[sledge sem] Prove the Load and Store cases (mostly)
Summary:
This required some minor tweaks to how the semantics encode values into
and out of byte lists. The remaining problems have to do with how LLVM
globals are translated into llair. At the moment, llair semantic's state
keeps a mapping for globals to their addresses, following the LLVM
semantics. However, it is not used because the translation (following
the code in frontend.ml) translates LLVM globals into llair locals,
which the llair semantics isn't set up to handle.

Reviewed By: jberdine

Differential Revision: D17930787

fbshipit-source-id: 06c6368e0

sledge/semantics/llairScript.sml
@@ -314,6 +314,7 @@ End
 (* BEGIN Functions to interface to the generic memory model *)
 Definition type_to_shape_def:
   (type_to_shape (IntegerT n) = Flat (sizeof (IntegerT n)) (IntegerT n)) ∧
+  (type_to_shape (PointerT t) = Flat (sizeof (PointerT t)) (PointerT t)) ∧
   (type_to_shape (ArrayT t n) = Array (type_to_shape t) n) ∧
   (type_to_shape (TupleT ts) = Tuple (map type_to_shape ts))
 Termination
@@ -324,7 +325,13 @@ Termination
 End
 
 Definition convert_value_def:
-  convert_value (IntegerT size) n = IntV (&n) size
+  (convert_value (IntegerT size) n =
+    if size = 1 then
+      IntV (if n = 0 then 0 else -1) size
+    else
+      n2i n size) ∧
+  (convert_value (PointerT t) n =
+    n2i n pointer_size)
 End
 
 Definition bytes_to_llair_value_def:
